backend/LTL.v
@@ -179,8 +179,7 @@ Definition undef_caller_save_regs (ls: locset) : locset :=
 Inductive stackframe : Type :=
   | Stackframe:
       forall (f: function)      (**r calling function *)
-        (cp: compartment)       (**r callee compartment *)
-        (sig: signature)        (**r signature of the callee, used to know the location of the return value *)
+             (sig: signature)   (**r signature of the callee, used to know the location of the return value *)
              (sp: val)          (**r stack pointer in calling function *)
              (ls: locset)       (**r location state in calling function *)
              (bb: bblock),      (**r continuation in calling function *)
@@ -213,21 +212,15 @@ Inductive state : Type :=
   | Returnstate:
       forall (stack: list stackframe) (**r call stack *)
              (ls: locset)             (**r location state of callee *)
-             (m: mem),                 (**r memory state *)
+             (m: mem)                 (**r memory state *)
+             (cp: compartment),       (**r compartment we're returning from *)
       state.
 
 Definition call_comp (stack: list stackframe) : option compartment :=
   match stack with
   | nil => None
-  | Stackframe f _ _ _ _ _ :: _ => Some (comp_of f)
+  | Stackframe f _ _ _ _ :: _ => Some (comp_of f)
   end.
-
-Definition callee_comp (stack: list stackframe) : option compartment :=
-  match stack with
-  | nil => None
-  | Stackframe _ cp _ _ _ _ :: _ => Some cp
-  end.
-
 
 Section RELSEM.
 
@@ -293,13 +286,13 @@ Qed.
 Definition parent_locset (stack: list stackframe) : locset :=
   match stack with
   | nil => Locmap.init Vundef
-  | Stackframe f _ _ sp ls bb :: stack' => ls
+  | Stackframe f _ sp ls bb :: stack' => ls
   end.
 
 Definition parent_signature (stack: list stackframe) : signature :=
   match stack with
   | nil => signature_main
-  | Stackframe _ _ sig _ _ _ :: stack' => sig
+  | Stackframe _ sig _ _ _ :: stack' => sig
   end.
 
 Inductive step: state -> trace -> state -> Prop :=
@@ -346,7 +339,7 @@ Inductive step: state -> trace -> state -> Prop :=
           List.Forall not_ptr args),
       forall (EV: call_trace ge (comp_of f) (comp_of fd) vf args (sig_args sig) t),
       step (Block s f sp (Lcall sig ros :: bb) rs m)
-        t (Callstate (Stackframe f (comp_of fd) sig sp rs bb :: s) fd sig rs m)
+        t (Callstate (Stackframe f sig sp rs bb :: s) fd sig rs m)
   | exec_Ltailcall: forall s f sp sig ros bb rs m fd rs' m',
       rs' = return_regs (parent_locset s) rs ->
       find_function ros rs' = Some fd ->
@@ -384,7 +377,7 @@ Inductive step: state -> trace -> state -> Prop :=
                retrs =
                  return_regs_ext (parent_locset s) rs (parent_signature s)),
       step (Block s f (Vptr sp Ptrofs.zero) (Lreturn :: bb) rs m)
-        E0 (Returnstate s retrs m')
+        E0 (Returnstate s retrs m' (comp_of f))
   | exec_function_internal: forall s f rs m m' sp callrs sig rs',
       Mem.alloc m (comp_of f) 0 f.(fn_stacksize) = (m', sp) ->
       forall (CALLREGS:
@@ -398,13 +391,13 @@ Inductive step: state -> trace -> state -> Prop :=
       external_call ef ge args m t res m' ->
       rs' = Locmap.setpair (loc_result (ef_sig ef)) res (undef_caller_save_regs rs) ->
       step (Callstate s (External ef) sig rs m)
-         t (Returnstate s rs' m')
+         t (Returnstate s rs' m' (comp_of ef))
   | exec_return: forall f sp rs1 bb s rs m cp sig t,
       forall (NO_CROSS_PTR:
           Genv.type_of_call (comp_of f) cp = Genv.CrossCompartmentCall ->
           not_ptr (Locmap.getpair (map_rpair R (loc_result sig)) rs)),
       forall (EV: return_trace ge (comp_of f) cp (Locmap.getpair (map_rpair R (loc_result sig)) rs) (sig_res sig) t),
-      step (Returnstate (Stackframe f cp sig sp rs1 bb :: s) rs m)
+      step (Returnstate (Stackframe f sig sp rs1 bb :: s) rs m cp)
         t (Block s f sp bb rs m).
 
 End RELSEM.
@@ -424,9 +417,9 @@ Inductive initial_state (p: program): state -> Prop :=
       initial_state p (Callstate nil f signature_main (Locmap.init Vundef) m0).
 
 Inductive final_state: state -> int -> Prop :=
-  | final_state_intro: forall rs m retcode,
+  | final_state_intro: forall rs m retcode cp,
       Locmap.getpair (map_rpair R (loc_result signature_main)) rs = Vint retcode ->
-      final_state (Returnstate nil rs m) retcode.
+      final_state (Returnstate nil rs m cp) retcode.
 
 Definition semantics (p: program) :=
   Semantics step (initial_state p) final_state (Genv.globalenv p).
